WIP: Remove reflexivity from Instantaneous.Execution

src/ReactorModel/Execution/Progress.lean
@@ -1,4 +1,5 @@
 import ReactorModel.Execution.Trace
+import ReactorModel.Determinism.ExecutionStep
 
 open ReactorType
 
@@ -14,13 +15,27 @@ structure State.Terminal (s : State α) : Prop where
   closed  : s.Closed
   no_next : ∀ g, ¬s.NextTag g
 
+theorem State.Terminal.not_of_not_closed {s : State α} (h : ¬s.Closed) : ¬State.Terminal s :=
+  (h ·.closed)
+
 -- A reactor has the progress property, if from any nonterminal state based at that reactor, we can 
 -- perform an execution step.
--- TODO: This isn't exactly what we want. The freshness condition is too restrictive.
 def Progress (rtr : α) : Prop :=
-  ∀ {s : State α}, (s.rtr = rtr) → (s.progress = ∅) → ¬s.Terminal → (∃ s', s ⇓ s')    
+  ∀ s, (s.rtr = rtr) → ¬s.Terminal → (∃ s', Nonempty $ s ⇓ s')    
 
-theorem Progress.iff_deps_acyclic {rtr : α} : (Progress rtr) ↔ (Dependency.Acyclic rtr) :=
-  sorry
+theorem Progress.iff_deps_acyclic {rtr : α} : (Progress rtr) ↔ (Dependency.Acyclic rtr) := by
+  simp [Dependency.Acyclic.iff_mem_acyclic]
+  constructor <;> intro h
+  case mp =>
+    intro rcn hm
+    let s : State α := { rtr, tag := 0, progress := ∅ }
+    have hc : ¬s.Closed := sorry -- for nontrivial state: follows from progress = ∅.
+    have ⟨_, ⟨e⟩⟩ := h s rfl (State.Terminal.not_of_not_closed hc)
+    replace e := e.resolve_close hc 
+    exact e.acyclic $ e.progress_empty_mem_rcns_iff rfl |>.mpr hm
+  case mpr =>
+    sorry
+    -- Perhaps you can avoid proving directly that you can perform clearing ports by using a proof by
+    -- contradiction.
 
 end Execution
