src/ReactorModel/Determinism/InstantaneousExecution.lean
@@ -8,16 +8,26 @@ namespace Execution
  
 variable [ReactorType.Proper α] {s₁ s₂ : State α} in section
 
-theorem progress_not_mem_rcns (e : s₁ ⇓ᵢ* s₂) (h : rcn ∈ s₁.progress) : rcn ∉ e.rcns := by
-  induction e <;> simp [rcns, not_or]
+theorem acyclic (e : s₁ ⇓ᵢ+ s₂) (h : rcn ∈ e.rcns) : rcn ≮[s₁.rtr] rcn := by
+  induction e <;> simp [rcns] at h <;> try cases ‹_ ∨ _›   
+  case single e           => exact h ▸ e.acyclic
+  case trans.inl e _ _ h  => exact h ▸ e.acyclic
+  case trans.inr e _ hi h => exact (hi h).equiv (ReactorType.Equivalent.symm e.equiv)
+
+theorem progress_not_mem_rcns (e : s₁ ⇓ᵢ+ s₂) (h : rcn ∈ s₁.progress) : rcn ∉ e.rcns := by
+  induction e <;> simp [rcns]
+  case single e =>
+    sorry
   case trans e e' hi =>
     simp [hi $ e.progress_monotonic h]
     intro hc
     exact e.rcn_not_mem_progress $ hc ▸ h
 
-theorem mem_progress_iff (e : s₁ ⇓ᵢ* s₂) : 
+theorem mem_progress_iff (e : s₁ ⇓ᵢ+ s₂) : 
     (rcn ∈ s₂.progress) ↔ (rcn ∈ e.rcns ∨ rcn ∈ s₁.progress) := by
   induction e <;> simp [rcns]
+  case single =>
+    sorry
   case trans s₁ s₂ s₃ e e' hi => 
     simp [hi]
     constructor <;> intro
@@ -25,17 +35,17 @@ theorem mem_progress_iff (e : s₁ ⇓ᵢ* s₂) :
     case mp.inr h      => cases e.mem_progress_iff.mp h <;> simp [*]
     case mpr.inl.inl h => simp [e.rcn_mem_progress]
     case mpr.inr h     => simp [e.progress_monotonic h]
- 
+
 -- Corollary of `InstExecution.mem_progress_iff`.
-theorem rcns_mem_progress (e : s₁ ⇓ᵢ* s₂) (h : rcn ∈ e.rcns) : rcn ∈ s₂.progress := 
+theorem rcns_mem_progress (e : s₁ ⇓ᵢ+ s₂) (h : rcn ∈ e.rcns) : rcn ∈ s₂.progress := 
   e.mem_progress_iff.mpr $ .inl h
 
-theorem rcns_nodup {s₁ s₂ : State α} : (e : s₁ ⇓ᵢ* s₂) → e.rcns.Nodup
-  | refl       => List.nodup_nil
+theorem rcns_nodup {s₁ s₂ : State α} : (e : s₁ ⇓ᵢ+ s₂) → e.rcns.Nodup
+  | single _   => List.nodup_singleton _
   | trans e e' => List.nodup_cons.mpr ⟨e'.progress_not_mem_rcns e.rcn_mem_progress, e'.rcns_nodup⟩
 
 theorem progress_eq_rcns_perm 
-    (e₁ : s ⇓ᵢ* s₁) (e₂ : s ⇓ᵢ* s₂) (hp : s₁.progress = s₂.progress) : e₁.rcns ~ e₂.rcns := by
+    (e₁ : s ⇓ᵢ+ s₁) (e₂ : s ⇓ᵢ+ s₂) (hp : s₁.progress = s₂.progress) : e₁.rcns ~ e₂.rcns := by
   apply List.perm_ext e₁.rcns_nodup e₂.rcns_nodup |>.mpr
   intro rcn
   by_cases hc : rcn ∈ s.progress
@@ -45,45 +55,48 @@ theorem progress_eq_rcns_perm
     case mp  => exact e₂.mem_progress_iff.mp (hp ▸ e₁.rcns_mem_progress hm) |>.resolve_right hc
     case mpr => exact e₁.mem_progress_iff.mp (hp ▸ e₂.rcns_mem_progress hm) |>.resolve_right hc
 
-theorem preserves_tag {s₁ s₂ : State α} : (s₁ ⇓ᵢ* s₂) → s₁.tag = s₂.tag
-  | refl => rfl
+theorem preserves_tag {s₁ s₂ : State α} : (s₁ ⇓ᵢ+ s₂) → s₁.tag = s₂.tag
+  | single e   => e.preserves_tag
   | trans e e' => e.preserves_tag.trans e'.preserves_tag
 
-theorem rcns_trans_eq_cons (e₁ : s ⇓ᵢ s₁) (e₂ : s₁ ⇓ᵢ* s₂) : 
+theorem rcns_trans_eq_cons (e₁ : s ⇓ᵢ s₁) (e₂ : s₁ ⇓ᵢ+ s₂) : 
     (trans e₁ e₂).rcns = e₁.rcn :: e₂.rcns := by
   simp [rcns, Step.rcn]
 
 theorem progress_eq {s₁ s₂ : State α} : 
-    (e : s₁ ⇓ᵢ* s₂) → s₂.progress = s₁.progress ∪ { i | i ∈ e.rcns }
-  | refl => by simp [rcns]
+    (e : s₁ ⇓ᵢ+ s₂) → s₂.progress = s₁.progress ∪ { i | i ∈ e.rcns }
+  | single e => by 
+    simp [rcns]
+    exact e.progress_eq
   | trans e e' => by 
     simp [e.progress_eq ▸ e'.progress_eq, rcns_trans_eq_cons]
     apply Set.insert_union'
 
-theorem mem_rcns_not_mem_progress (e : s₁ ⇓ᵢ* s₂) (h : rcn ∈ e.rcns) : rcn ∉ s₁.progress := by
+theorem mem_rcns_not_mem_progress (e : s₁ ⇓ᵢ+ s₂) (h : rcn ∈ e.rcns) : rcn ∉ s₁.progress := by
   induction e
-  case refl => contradiction
+  case single => 
+    sorry -- contradiction
   case trans e e' hi =>
     cases e'.rcns_trans_eq_cons e ▸ h
     case head   => exact e.rcn_not_mem_progress
     case tail h => exact mt e.progress_monotonic (hi h)
 
-theorem mem_rcns_iff (e : s₁ ⇓ᵢ* s₂) : rcn ∈ e.rcns ↔ (rcn ∈ s₂.progress ∧ rcn ∉ s₁.progress) := by
+theorem mem_rcns_iff (e : s₁ ⇓ᵢ+ s₂) : rcn ∈ e.rcns ↔ (rcn ∈ s₂.progress ∧ rcn ∉ s₁.progress) := by
   simp [e.progress_eq, s₁.mem_record'_progress_iff e.rcns rcn, or_and_right]
   exact e.mem_rcns_not_mem_progress
 
-theorem equiv {s₁ s₂ : State α} : (s₁ ⇓ᵢ* s₂) → s₁.rtr ≈ s₂.rtr
-  | refl       => .refl _
+theorem equiv {s₁ s₂ : State α} : (s₁ ⇓ᵢ+ s₂) → s₁.rtr ≈ s₂.rtr
+  | single e   => e.equiv
   | trans e e' => ReactorType.Equivalent.trans e.equiv e'.equiv
 
-theorem head_minimal (e : s₁ ⇓ᵢ s₂) (e' : s₂ ⇓ᵢ* s₃) : (e.rcn :: e'.rcns) ≮[s₁.rtr] e.rcn := by
+theorem head_minimal (e : s₁ ⇓ᵢ s₂) (e' : s₂ ⇓ᵢ+ s₃) : (e.rcn :: e'.rcns) ≮[s₁.rtr] e.rcn := by
   by_contra hc
   simp [Minimal] at hc
   have ⟨_, hm, h⟩ := hc e.acyclic
   replace hc := mt e.progress_monotonic $ e'.mem_rcns_not_mem_progress hm
   exact hc $ e.allows_rcn.deps h
 
-theorem head_not_mem_tail (e : s₁ ⇓ᵢ s₂) (e' : s₂ ⇓ᵢ* s₃) (h : i ∈ e'.rcns) : e.rcn ≠ i := by
+theorem head_not_mem_tail (e : s₁ ⇓ᵢ s₂) (e' : s₂ ⇓ᵢ+ s₃) (h : i ∈ e'.rcns) : e.rcn ≠ i := by
   intro hc
   have := trans e e' |>.rcns_nodup
   have := hc.symm ▸ List.not_nodup_cons_of_mem h
@@ -95,9 +108,11 @@ variable [ReactorType.Proper α] {s₁ s₂ : State α}
 
 -- The core lemma for `prepend_minimal`.
 theorem cons_prepend_minimal 
-    (e : s₁ ⇓ᵢ s₂) (e' : s₂ ⇓ᵢ* s₃) (hm : i ∈ e'.rcns) (hr : (e.rcn :: e'.rcns) ≮[s₁.rtr] i) : 
-    ∃ f : s₁ ⇓ᵢ* s₃, f.rcns = i :: e.rcn :: (e'.rcns.erase i) := by
+    (e : s₁ ⇓ᵢ s₂) (e' : s₂ ⇓ᵢ+ s₃) (hm : i ∈ e'.rcns) (hr : (e.rcn :: e'.rcns) ≮[s₁.rtr] i) : 
+    ∃ f : s₁ ⇓ᵢ+ s₃, f.rcns = i :: e.rcn :: (e'.rcns.erase i) := by
   induction e' generalizing s₁ <;> simp [rcns] at *
+  case single =>
+    sorry
   case trans s₁ s₂ s₄ e' e'' hi =>
     cases hm
     case inl hm =>
@@ -114,9 +129,11 @@ theorem cons_prepend_minimal
         exists trans f $ trans f' f''
         simp [rcns, hf₁, h₁, hf₂, h₂, e''.rcns.erase_cons_tail $ head_not_mem_tail e' e'' hm]
 
-theorem prepend_minimal (e : s₁ ⇓ᵢ* s₂) (hm : i ∈ e.rcns) (hr : e.rcns ≮[s₁.rtr] i) :
-    ∃ (e' : s₁ ⇓ᵢ* s₂), e'.rcns = i :: (e.rcns.erase i) := by
-  cases e <;> simp [rcns] at *; cases ‹_ ∨ _› 
+theorem prepend_minimal (e : s₁ ⇓ᵢ+ s₂) (hm : i ∈ e.rcns) (hr : e.rcns ≮[s₁.rtr] i) :
+    ∃ (e' : s₁ ⇓ᵢ+ s₂), e'.rcns = i :: (e.rcns.erase i) := by
+  cases e <;> (simp [rcns] at *; try cases ‹_ ∨ _›)
+  case single =>
+    sorry
   case trans.inl e e' h =>
     exists trans e e'
     simp [rcns, h]
@@ -124,14 +141,17 @@ theorem prepend_minimal (e : s₁ ⇓ᵢ* s₂) (hm : i ∈ e.rcns) (hr : e.rcns
     exact e'.rcns.erase_cons_tail (head_not_mem_tail e e' h) ▸ cons_prepend_minimal e e' h hr
         
 theorem rcns_perm_deterministic 
-    (e₁ : s ⇓ᵢ* s₁) (e₂ : s ⇓ᵢ* s₂) (hp : e₁.rcns ~ e₂.rcns) : s₁.rtr = s₂.rtr := by
+    (e₁ : s ⇓ᵢ+ s₁) (e₂ : s ⇓ᵢ+ s₂) (hp : e₁.rcns ~ e₂.rcns) : s₁.rtr = s₂.rtr := by
   induction e₁
-  case refl => cases e₂ <;> simp [rcns] at hp ⊢ 
+  case single => 
+    sorry -- cases e₂ <;> simp [rcns] at hp ⊢ 
   case trans s sₘ₁ s₁ e₁ e₁' hi =>
     have hm := hp.mem_iff.mp $ List.mem_cons_self _ _
     have hm' := e₁'.head_minimal e₁ |>.perm hp
     have ⟨e₂, he₂⟩ := e₂.prepend_minimal hm hm'
     cases e₂ <;> simp [rcns] at he₂
+    case single =>
+      sorry
     case trans sₘ₂ e₂ e₂' =>
       have ⟨h, h'⟩ := he₂ 
       cases e₁.deterministic e₂ h.symm
@@ -140,7 +160,7 @@ theorem rcns_perm_deterministic
       exact List.perm_cons _ |>.mp (hp.trans $ List.perm_cons_erase hm)
 
 protected theorem deterministic 
-    (e₁ : s ⇓ᵢ* s₁) (e₂ : s ⇓ᵢ* s₂) (ht : s₁.tag = s₂.tag) (hp : s₁.progress = s₂.progress) : 
+    (e₁ : s ⇓ᵢ+ s₁) (e₂ : s ⇓ᵢ+ s₂) (ht : s₁.tag = s₂.tag) (hp : s₁.progress = s₂.progress) : 
     s₁ = s₂ := by
   ext1 <;> try assumption
   exact rcns_perm_deterministic e₁ e₂ $ progress_eq_rcns_perm e₁ e₂ hp
