src/ReactorModel/Execution/Dependency.lean
@@ -30,7 +30,7 @@ notation i₁ " <[" rtr "] " i₂ => Dependency rtr i₁ i₂
 namespace Dependency
 
 open Indexable Equivalent
-variable [Indexable α] {rtr₁ : α}
+variable [Indexable α] {rtr rtr₁ : α}
  
 theorem equiv (e : rtr₁ ≈ rtr₂) (d : j₁ <[rtr₂] j₂) : j₁ <[rtr₁] j₂ := by
   induction d with
@@ -40,12 +40,12 @@ theorem equiv (e : rtr₁ ≈ rtr₂) (d : j₁ <[rtr₂] j₂) : j₁ <[rtr₁]
     have ⟨_, h₁'⟩ := obj?_some_iff e |>.mpr ⟨_, h₁⟩
     have e := Equivalent.obj?_rtr_equiv e h₁' h₁
     exact prio h₁' (get?_rcn_eq e ▸ h₂) (get?_rcn_eq e ▸ h₃) ‹_› ‹_›
+  | depOverlap h₁ h₂ => 
+    exact depOverlap (e.obj?_rcn_eq.symm ▸ h₁) (e.obj?_rcn_eq.symm ▸ h₂) ‹_› ‹_› ‹_›
   | mutNorm h₁ h₂ h₃ => 
     have ⟨_, h₁'⟩ := obj?_some_iff e |>.mpr ⟨_, h₁⟩  
     have e := Equivalent.obj?_rtr_equiv e h₁' h₁
     exact mutNorm h₁' (get?_rcn_eq e ▸ h₂) (get?_rcn_eq e ▸ h₃) ‹_› ‹_›
-  | depOverlap h₁ h₂ => 
-    exact depOverlap (e.obj?_rcn_eq.symm ▸ h₁) (e.obj?_rcn_eq.symm ▸ h₂) ‹_› ‹_› ‹_›
   | mutNest h₁ h₂ h₃ _ h₄ => 
     have ⟨_, h₁'⟩ := e.obj?_some_iff.mpr ⟨_, h₁⟩  
     have e := Equivalent.obj?_rtr_equiv e h₁' h₁
@@ -55,11 +55,23 @@ theorem equiv (e : rtr₁ ≈ rtr₂) (d : j₁ <[rtr₂] j₂) : j₁ <[rtr₁]
   | trans _ _ d₁ d₂ => 
     exact trans d₁ d₂
 
+theorem mem₁ (d : rcn₁ <[rtr] rcn₂) : rcn₁ ∈ rtr[.rcn] := by
+  induction d <;> try exact Partial.mem_iff.mpr ⟨_, obj?_some_extend ‹_› ‹_›⟩ 
+  case depOverlap => exact Partial.mem_iff.mpr ⟨_, ‹_›⟩ 
+  case trans => assumption
+  
 def Acyclic (rtr : α) : Prop :=
   ∀ i, ¬(i <[rtr] i)
 
 theorem Acyclic.equiv (e : rtr₁ ≈ rtr₂) (a : Acyclic rtr₁) : Acyclic rtr₂ :=
   (a · $ ·.equiv e)
+
+theorem Acyclic.iff_mem_acyclic {rtr : α} : (Acyclic rtr) ↔ (∀ i ∈ rtr[.rcn], ¬(i <[rtr] i)) := by
+  apply not_iff_not.mp
+  simp [Acyclic]
+  constructor <;> intro ⟨d, h⟩  
+  case mp  => exact ⟨_, h.mem₁, h⟩
+  case mpr => exact ⟨_, h.right⟩ 
 
 end Dependency
 end ReactorType
